

# Chapter 1

## Linear Regression

### Ordinary Least Squares

**Theorem 1.0.1** (Uniqueness of the Least Squares Solution). *Let  $\Phi \in \mathbb{R}^{N \times M}$  denote the design matrix and  $t \in \mathbb{R}^N$  the target vector. Consider the least squares cost function*

$$E(w) = \frac{1}{2} \|t - \Phi w\|^2.$$

Then:

- (i) *The function  $E(w)$  is convex in  $w$ .*
- (ii) *If  $\Phi^\top \Phi$  is invertible (i.e.,  $\text{rank}(\Phi) = M$ ), then  $E(w)$  is strictly convex and admits a unique minimizer*

$$w^* = (\Phi^\top \Phi)^{-1} \Phi^\top t.$$

- (iii) *If  $\Phi^\top \Phi$  is singular, the minimizer is not unique; all minimizers are of the form*

$$w = w_0 + v, \quad v \in \text{Null}(\Phi),$$

where  $w_0$  is any particular solution to the normal equations  $\Phi^\top \Phi w = \Phi^\top t$ .

*Proof.* We begin by expanding the objective:

$$E(w) = \frac{1}{2} (t - \Phi w)^\top (t - \Phi w) = \frac{1}{2} (t^\top t - 2t^\top \Phi w + w^\top \Phi^\top \Phi w).$$

- (1) Gradient and Stationary Point:** The gradient of  $E(w)$  with respect to  $w$  is

$$\nabla_w E(w) = -\Phi^\top t + \Phi^\top \Phi w.$$

Setting  $\nabla_w E(w) = 0$  yields the *normal equations*

$$\Phi^\top \Phi w = \Phi^\top t.$$

- (2) Hessian and Convexity:** The Hessian of  $E(w)$  is

$$H = \nabla_w^2 E(w) = \Phi^\top \Phi.$$

For any nonzero vector  $z \in \mathbb{R}^M$ ,

$$z^\top H z = z^\top \Phi^\top \Phi z = \|\Phi z\|^2 \geq 0,$$

hence  $H$  is positive semidefinite, implying  $E(w)$  is convex.

If  $\Phi$  has full column rank ( $\text{rank}(\Phi) = M$ ), then  $\Phi^\top \Phi$  is positive definite, and

$$z^\top H z = 0 \quad \Leftrightarrow \quad z = 0,$$

so  $E(w)$  is strictly convex. A strictly convex function has a unique minimizer, obtained by solving (1):

$$w^* = (\Phi^\top \Phi)^{-1} \Phi^\top t.$$

- (3) Non-uniqueness for Rank-Deficient  $\Phi$ :** If  $\Phi^\top \Phi$  is singular, there exist nonzero vectors  $v$  such that  $\Phi v = 0$ . For any particular solution  $w_0$  satisfying (1), we have

$$\Phi^\top \Phi (w_0 + v) = \Phi^\top \Phi w_0 + \Phi^\top \Phi v = \Phi^\top t,$$

since  $\Phi v = 0$ . Thus, every vector  $w = w_0 + v$ , with  $v \in \text{Null}(\Phi)$ , minimizes  $E(w)$ . The minimal-norm solution among them is given by the Moore–Penrose pseudoinverse:

$$w^* = \Phi^+ t.$$

- (4) Conclusion:** The cost  $E(w)$  is convex for all  $\Phi$ , and strictly convex (hence uniquely minimized) iff  $\Phi^\top \Phi$  is invertible.  $\square$

**Theorem 1.0.2** (Unbiasedness of the OLS Estimator). *Assume the linear regression model*

$$t = \Phi w + \varepsilon,$$

- (1) *where  $\Phi \in \mathbb{R}^{N \times M}$  is the design matrix,  $w \in \mathbb{R}^M$  the true parameter vector, and the noise satisfies  $\mathbb{E}[\varepsilon] = 0$  and  $\text{Cov}(\varepsilon) = \sigma^2 I$ . Assume further that  $\Phi^\top \Phi$  is invertible. Then the ordinary least squares estimator*

$$\hat{w} = (\Phi^\top \Phi)^{-1} \Phi^\top t$$

*is an unbiased estimator of  $w$ , i.e.*

$$\mathbb{E}[\hat{w}] = w.$$

*Proof.* By the model,

$$t = \Phi w + \varepsilon.$$

Substitute into the estimator:

$$\hat{w} = (\Phi^\top \Phi)^{-1} \Phi^\top t = (\Phi^\top \Phi)^{-1} \Phi^\top (\Phi w + \varepsilon).$$

Distribute terms:

$$\hat{w} = (\Phi^\top \Phi)^{-1} \Phi^\top \Phi w + (\Phi^\top \Phi)^{-1} \Phi^\top \varepsilon.$$

Since  $(\Phi^\top \Phi)^{-1} \Phi^\top \Phi = I_M$ , this simplifies to

$$\hat{w} = w + (\Phi^\top \Phi)^{-1} \Phi^\top \varepsilon.$$

Take expectation using linearity and  $\mathbb{E}[\varepsilon] = 0$ :

$$\mathbb{E}[\hat{w}] = \mathbb{E}[w + (\Phi^\top \Phi)^{-1} \Phi^\top \varepsilon] = w + (\Phi^\top \Phi)^{-1} \Phi^\top \mathbb{E}[\varepsilon] = w + (\Phi^\top \Phi)^{-1} \Phi^\top 0 = w.$$

Thus  $\hat{w}$  is unbiased.

**Corollary 1.0.3.** *Under the same assumptions,*

$$\text{Cov}(\hat{w}) = \sigma^2 (\Phi^\top \Phi)^{-1}.$$

*Proof.* From  $\hat{w} = w + (\Phi^\top \Phi)^{-1} \Phi^\top \varepsilon$  and  $\text{Cov}(\varepsilon) = \sigma^2 I$ ,

$$\text{Cov}(\hat{w}) = (\Phi^\top \Phi)^{-1} \Phi^\top \text{Cov}(\varepsilon) \Phi (\Phi^\top \Phi)^{-1} = \sigma^2 (\Phi^\top \Phi)^{-1} \Phi^\top \Phi (\Phi^\top \Phi)^{-1} = \sigma^2 (\Phi^\top \Phi)^{-1}.$$

**Theorem 1.0.4** (Covariance of the OLS Estimator). *Under the linear regression model*

$$t = \Phi w + \varepsilon, \quad \mathbb{E}[\varepsilon] = 0, \quad \text{Cov}(\varepsilon) = \sigma^2 I,$$

*with  $\Phi \in \mathbb{R}^{N \times M}$  of full column rank, the ordinary least squares estimator*

$$\hat{w} = (\Phi^\top \Phi)^{-1} \Phi^\top t$$

*has covariance matrix*

$$\text{Cov}(\hat{w}) = \sigma^2 (\Phi^\top \Phi)^{-1}.$$

*Proof.* From the model  $t = \Phi w + \varepsilon$ ,

$$\hat{w} = (\Phi^\top \Phi)^{-1} \Phi^\top t = (\Phi^\top \Phi)^{-1} \Phi^\top (\Phi w + \varepsilon) = w + (\Phi^\top \Phi)^{-1} \Phi^\top \varepsilon.$$

Subtract the expectation  $\mathbb{E}[\hat{w}] = w$  to get the deviation:

$$\hat{w} - \mathbb{E}[\hat{w}] = (\Phi^\top \Phi)^{-1} \Phi^\top \varepsilon.$$

Now compute the covariance:

$$\begin{aligned} \text{Cov}(\hat{w}) &= \mathbb{E}[(\hat{w} - \mathbb{E}[\hat{w}])(\hat{w} - \mathbb{E}[\hat{w}])^\top] \\ &= \mathbb{E}[(\Phi^\top \Phi)^{-1} \Phi^\top \varepsilon \varepsilon^\top \Phi (\Phi^\top \Phi)^{-1}]. \end{aligned}$$

Using  $\text{Cov}(\varepsilon) = \sigma^2 I$  and the linearity of expectation:

$$\text{Cov}(\hat{w}) = (\Phi^\top \Phi)^{-1} \Phi^\top (\sigma^2 I) \Phi (\Phi^\top \Phi)^{-1} = \sigma^2 (\Phi^\top \Phi)^{-1} \Phi^\top \Phi (\Phi^\top \Phi)^{-1}.$$

Simplifying:

$$\boxed{\text{Cov}(\hat{w}) = \sigma^2 (\Phi^\top \Phi)^{-1}}.$$

**Theorem 1.0.5** (Gauss–Markov Theorem). *Consider the linear model*

$$t = \Phi w + \varepsilon,$$

*with  $\Phi \in \mathbb{R}^{N \times M}$  of full column rank,  $\mathbb{E}[\varepsilon] = 0$ , and  $\text{Cov}(\varepsilon) = \sigma^2 I$ . Let  $\hat{w}_{\text{OLS}} = (\Phi^\top \Phi)^{-1} \Phi^\top t$  denote the ordinary least squares estimator. Then  $\hat{w}_{\text{OLS}}$  is the Best Linear Unbiased Estimator (BLUE): for any other linear unbiased estimator of the form  $\tilde{w} = Ct$  (with constant matrix  $C \in \mathbb{R}^{M \times N}$  such that  $\mathbb{E}[\tilde{w}] = w$ ), we have*

$$\text{Cov}(\tilde{w}) - \text{Cov}(\hat{w}_{\text{OLS}}) \succeq 0,$$

*i.e. the matrix difference is positive semidefinite. Equivalently, every componentwise variance of  $\tilde{w}$  is at least that of  $\hat{w}_{\text{OLS}}$ .*

□ *Proof.* Let  $\tilde{w}$  be any linear estimator of the form  $\tilde{w} = Ct$  for a fixed matrix  $C \in \mathbb{R}^{M \times N}$ . The unbiasedness condition  $\mathbb{E}[\tilde{w}] = w$  requires

$$\mathbb{E}[Ct] = C\mathbb{E}[t] = C\Phi w = w \quad \text{for all } w,$$

hence

$$C\Phi = I_M. \tag{1}$$

□ Write the OLS estimator as

$$\hat{w} \equiv \hat{w}_{\text{OLS}} = (\Phi^\top \Phi)^{-1} \Phi^\top t.$$

Define the matrix difference

$$A := C - (\Phi^\top \Phi)^{-1} \Phi^\top.$$

Using (1) and the identity  $((\Phi^\top \Phi)^{-1} \Phi^\top) \Phi = I_M$ , we obtain

$$A\Phi = C\Phi - (\Phi^\top \Phi)^{-1} \Phi^\top \Phi = I_M - I_M = 0.$$

Thus

$$A\Phi = 0 \quad \implies \quad A\Phi w = 0 \quad \text{for all } w.$$

Now express  $\tilde{w}$  in terms of  $\hat{w}$  and  $A$ :

$$\tilde{w} = Ct = ((\Phi^\top \Phi)^{-1} \Phi^\top + A)t = \hat{w} + At.$$

Subtracting expectations (and using  $\mathbb{E}[\hat{w}] = \mathbb{E}[\tilde{w}] = w$ ) gives the zero-mean deviations

$$\tilde{w} - w = (\hat{w} - w) + A\varepsilon,$$

since  $t = \Phi w + \varepsilon$  and  $A\Phi w = 0$ .

Compute the covariance matrices. Using  $\text{Cov}(\varepsilon) = \sigma^2 I$  and independence of deterministic matrices from  $\varepsilon$ ,

$$\begin{aligned} \text{Cov}(\tilde{w}) &= \mathbb{E}[(\tilde{w} - w)(\tilde{w} - w)^\top] \\ &= \mathbb{E}[(\hat{w} - w + A\varepsilon)(\hat{w} - w + A\varepsilon)^\top] \\ &= \text{Cov}(\hat{w}) + A\mathbb{E}[\varepsilon\varepsilon^\top]A^\top + \mathbb{E}[(\hat{w} - w)\varepsilon^\top]A^\top + A\mathbb{E}[(\hat{w} - w)^\top\varepsilon]. \end{aligned}$$

□

But  $\hat{w} - w = (\Phi^\top \Phi)^{-1} \Phi^\top \varepsilon$  is linear in  $\varepsilon$ , so

$$\mathbb{E}[(\hat{w} - w)\varepsilon^\top] = (\Phi^\top \Phi)^{-1} \Phi^\top \mathbb{E}[\varepsilon \varepsilon^\top] = (\Phi^\top \Phi)^{-1} \Phi^\top (\sigma^2 I) = \sigma^2 (\Phi^\top \Phi)^{-1} \Phi^\top.$$

Since  $A\Phi = 0$ , we have

$$\mathbb{E}[(\hat{w} - w)\varepsilon^\top] A^\top = \sigma^2 (\Phi^\top \Phi)^{-1} \Phi^\top A^\top = \sigma^2 (\Phi^\top \Phi)^{-1} (\Phi^\top A^\top) = \sigma^2 (\Phi^\top \Phi)^{-1} (A\Phi)^\top = 0.$$

Similarly the other cross term  $A \mathbb{E}[\varepsilon(\hat{w} - w)^\top]$  vanishes. Thus the covariance simplifies to

$$\text{Cov}(\tilde{w}) = \text{Cov}(\hat{w}) + A \mathbb{E}[\varepsilon \varepsilon^\top] A^\top = \text{Cov}(\hat{w}) + \sigma^2 A A^\top.$$

Therefore

$$\text{Cov}(\tilde{w}) - \text{Cov}(\hat{w}) = \sigma^2 A A^\top.$$

But  $\sigma^2 A A^\top$  is positive semidefinite (for any  $\sigma^2 \geq 0$  and any matrix  $A$ ), so

$$\text{Cov}(\tilde{w}) - \text{Cov}(\hat{w}) \succeq 0,$$

which proves that  $\hat{w}$  has the smallest covariance matrix among all linear unbiased estimators. This completes the proof.  $\square$

**Theorem 1.0.6** (Orthogonality of Residuals). *Let  $\Phi \in \mathbb{R}^{N \times M}$  be the design matrix and  $t \in \mathbb{R}^N$  the observed targets. Let  $\hat{w}$  be any solution of the normal equations*

$$\Phi^\top \Phi \hat{w} = \Phi^\top t.$$

*Define the residual vector  $r := t - \Phi \hat{w}$ . Then*

$$\Phi^\top r = 0,$$

*i.e.  $r$  is orthogonal to every column of  $\Phi$  (equivalently  $r$  is orthogonal to  $\text{col}(\Phi)$ ).*

*Proof.* Starting from the normal equations,

$$\Phi^\top \Phi \hat{w} = \Phi^\top t.$$

Rearrange terms to move  $\Phi^\top \Phi \hat{w}$  to the right-hand side:

$$\Phi^\top t - \Phi^\top \Phi \hat{w} = 0.$$

Factor  $\Phi^\top$ :

$$\Phi^\top (t - \Phi \hat{w}) = 0.$$

But  $t - \Phi \hat{w}$  is exactly the residual vector  $r$ , hence

$$\Phi^\top r = 0.$$

This shows each column of  $\Phi$  has zero inner product with  $r$ , i.e.  $r \perp \text{col}(\Phi)$ .  $\square$

**Corollary 1.0.7** (Hat Matrix and Residual Projection). *If  $\Phi$  has full column rank and  $\hat{w} = (\Phi^\top \Phi)^{-1} \Phi^\top t$ , define the hat (projection) matrix*

$$P := \Phi(\Phi^\top \Phi)^{-1} \Phi^\top.$$

*Then the fitted values are  $\hat{t} = Pt$  and the residual satisfies*

$$r = (I - P)t,$$

*with  $P^2 = P$  and  $P^\top = P$ . Consequently  $(I - P)$  is the orthogonal projector onto  $\text{col}(\Phi)^\perp$ , and  $r$  is the orthogonal projection of  $t$  onto that complement.*

*Proof.* Using  $\hat{w} = (\Phi^\top \Phi)^{-1} \Phi^\top t$  gives  $\hat{t} = \Phi \hat{w} = \Phi(\Phi^\top \Phi)^{-1} \Phi^\top t = Pt$ , so  $r = t - \hat{t} = (I - P)t$ . The identities  $P^2 = P$  and  $P^\top = P$  follow from straightforward algebra:

$$P^2 = \Phi(\Phi^\top \Phi)^{-1} \underbrace{\Phi^\top \Phi}_{=I} (\Phi^\top \Phi)^{-1} \Phi^\top = P, \quad P^\top = (\Phi(\Phi^\top \Phi)^{-1} \Phi^\top)^\top = \Phi(\Phi^\top \Phi)^{-1} \Phi^\top = P.$$

Thus  $P$  is an orthogonal projector onto  $\text{col}(\Phi)$  and  $(I - P)$  projects orthogonally onto its complement, so  $r$  lies in  $\text{col}(\Phi)^\perp$ .  $\square$

## Bayesian Linear Regression: Prior on $w$ and Predictive Distribution

### Bayesian Formulation

In Bayesian linear regression we treat the parameter vector  $w$  as a random variable and place a prior distribution on it. The generative model is:

$$t = \Phi w + \varepsilon, \quad \varepsilon \sim \mathcal{N}(0, \beta^{-1} I_N),$$

where  $\beta$  is the noise precision.

### Prior Distribution on $w$

We choose a zero-mean isotropic Gaussian prior:

$$p(w) = \mathcal{N}(w \mid 0, \alpha^{-1} I_M),$$

where  $\alpha$  is the prior precision. This encodes the belief that large weights are unlikely (acts as a regularizer).

### Likelihood

Conditioned on  $w$ , the likelihood of the data is:

$$p(t \mid \Phi, w, \beta) = \mathcal{N}(t \mid \Phi w, \beta^{-1} I_N).$$

### Posterior Distribution of $w$

By Bayes' theorem:

$$p(w \mid t, \Phi) \propto p(t \mid \Phi, w, \beta) p(w).$$

Because both prior and likelihood are Gaussian, the posterior is also Gaussian:

$$p(w \mid t, \Phi) = \mathcal{N}(w \mid m_N, S_N),$$

with posterior precision and covariance given by:

$$S_N^{-1} = \alpha I_M + \beta \Phi^\top \Phi, \quad S_N = (\alpha I_M + \beta \Phi^\top \Phi)^{-1},$$

and the posterior mean:

$$m_N = \beta S_N \Phi^\top t.$$

### Interpretation

- $m_N$  is the Bayes estimate of  $w$  (posterior mean).
- $S_N$  quantifies uncertainty in the weight estimates.
- As  $\alpha \rightarrow 0$  (weak prior),

$$m_N \rightarrow (\Phi^\top \Phi)^{-1} \Phi^\top t,$$

recovering the ordinary least squares solution.

## Predictive Distribution

For a new input  $x_*$  with feature vector  $\phi_* = \phi(x_*)$ , the predictive distribution integrates over the posterior uncertainty in  $w$ :

$$p(t_* | x_*, t, \Phi) = \int p(t_* | x_*, w, \beta) p(w | t, \Phi) dw.$$

The integrand is a product of two Gaussians, so the predictive distribution is Gaussian:

$$p(t_* | x_*, t, \Phi) = \mathcal{N}(t_* | m_N^\top \phi_*, \beta^{-1} + \phi_*^\top S_N \phi_*).$$

## Predictive Mean and Variance

**Predictive Mean:**

$$\mathbb{E}[t_* | x_*, t, \Phi] = m_N^\top \phi_*.$$

**Predictive Variance:**

$$\text{Var}(t_* | x_*, t, \Phi) = \underbrace{\beta^{-1}}_{\text{noise variance}} + \underbrace{\phi_*^\top S_N \phi_*}_{\text{model uncertainty}}.$$

Thus the predictive variance decomposes into:

- aleatoric noise (irreducible), and
- epistemic uncertainty (reduced with more data).

## Likelihood Derivation (Gaussian Noise) and MLEs

### 1. Single-observation likelihood

Assume the data generation model for a single observation:

$$t_n = w^\top \phi(x_n) + \varepsilon_n, \quad \varepsilon_n \sim \mathcal{N}(0, \beta^{-1}).$$

Then the conditional density (likelihood) for  $t_n$  given  $w$  is

$$p(t_n | x_n, w, \beta) = \mathcal{N}(t_n | w^\top \phi(x_n), \beta^{-1}) = \sqrt{\frac{\beta}{2\pi}} \exp\left(-\frac{\beta}{2}(t_n - w^\top \phi(x_n))^2\right).$$

### 2. Joint likelihood for the dataset

Assuming i.i.d. noise, the joint likelihood for all  $N$  observations is the product

$$p(t | \Phi, w, \beta) = \prod_{n=1}^N p(t_n | x_n, w, \beta) = \left(\frac{\beta}{2\pi}\right)^{N/2} \exp\left(-\frac{\beta}{2} \sum_{n=1}^N (t_n - w^\top \phi(x_n))^2\right).$$

Using matrix notation with  $\Phi \in \mathbb{R}^{N \times M}$  and  $t \in \mathbb{R}^N$ :

$$p(t | \Phi, w, \beta) = \left(\frac{\beta}{2\pi}\right)^{N/2} \exp\left(-\frac{\beta}{2} \|t - \Phi w\|^2\right).$$

### 3. Log-likelihood

The log-likelihood (more convenient for optimization) is

$$\ell(w, \beta) := \log p(t | \Phi, w, \beta) = \frac{N}{2} \log \beta - \frac{N}{2} \log(2\pi) - \frac{\beta}{2} \|t - \Phi w\|^2.$$

Dropping constants independent of the parameters when optimizing:

$$\ell(w, \beta) = \frac{N}{2} \log \beta - \frac{\beta}{2} \|t - \Phi w\|^2 + \text{const.}$$

### 4. MLE for $w$ (given $\beta$ )

Take gradient of the log-likelihood w.r.t.  $w$ :

$$\nabla_w \ell(w, \beta) = -\frac{\beta}{2} \cdot 2(-\Phi^\top)(t - \Phi w) = \beta \Phi^\top (t - \Phi w).$$

Set to zero for critical point:

$$\Phi^\top (t - \Phi w) = 0 \quad \Rightarrow \quad \Phi^\top \Phi w = \Phi^\top t.$$

If  $\Phi^\top \Phi$  is invertible, the MLE of  $w$  is

$$\hat{w}_{\text{MLE}} = (\Phi^\top \Phi)^{-1} \Phi^\top t$$

which is the ordinary least squares solution. Thus MLE = least squares under Gaussian noise.

### 5. MLE for noise precision $\beta$ (given $w$ )

Differentiate  $\ell$  w.r.t.  $\beta$ :

$$\frac{\partial \ell}{\partial \beta} = \frac{N}{2\beta} - \frac{1}{2} \|t - \Phi w\|^2.$$

Set equal to zero:

$$\frac{N}{2\beta} = \frac{1}{2} \|t - \Phi w\|^2 \quad \Rightarrow \quad \hat{\beta}_{\text{MLE}} = \frac{N}{\|t - \Phi w\|^2}.$$

If we substitute  $w = \hat{w}_{\text{MLE}}$  we get the MLE for  $\beta$ :

$$\hat{\beta}_{\text{MLE}} = \frac{N}{\|t - \Phi \hat{w}_{\text{MLE}}\|^2}.$$

Equivalently, the MLE for noise variance  $\sigma^2 = \beta^{-1}$  is

$$\hat{\sigma}_{\text{MLE}}^2 = \frac{1}{N} \|t - \Phi \hat{w}_{\text{MLE}}\|^2.$$

(For an unbiased estimator of  $\sigma^2$  divide by  $N - M$  instead of  $N$ .)

### 6. Negative log-likelihood and connection to MAP

The negative log-likelihood (up to additive constant) is

$$-\ell(w, \beta) \propto \frac{\beta}{2} \|t - \Phi w\|^2 - \frac{N}{2} \log \beta.$$

When combining with a Gaussian prior  $p(w) \propto \exp(-\frac{\alpha}{2} \|w\|^2)$ , the negative log-posterior (up to constants) becomes

$$-\log p(w | t) \propto \frac{\beta}{2} \|t - \Phi w\|^2 + \frac{\alpha}{2} \|w\|^2,$$

whose minimizer yields the MAP estimator. Dividing through by  $\beta$  and setting  $\lambda = \alpha/\beta$  gives the familiar ridge form:

$$\hat{w}_{\text{MAP}} = (\Phi^\top \Phi + \lambda I)^{-1} \Phi^\top t.$$

## Derivation of the Posterior with a Gaussian Prior (Completing the Square)

Assume the Gaussian likelihood and Gaussian prior:

$$p(t | w) \propto \exp\left(-\frac{\beta}{2}\|t - \Phi w\|^2\right), \quad p(w) \propto \exp\left(-\frac{\alpha}{2}\|w\|^2\right).$$

Posterior (unnormalized) by Bayes' rule:

$$p(w | t) \propto p(t | w) p(w) \propto \exp\left(-\frac{\beta}{2}\|t - \Phi w\|^2 - \frac{\alpha}{2}\|w\|^2\right).$$

**Expand the exponents (quadratic form in  $w$ ).**

$$\begin{aligned} & \frac{\beta}{2}\|t - \Phi w\|^2 + \frac{\alpha}{2}\|w\|^2 \\ &= \frac{\beta}{2}(t^\top t - 2t^\top \Phi w + w^\top \Phi^\top \Phi w) + \frac{\alpha}{2}w^\top w \\ &= \frac{1}{2}w^\top (\beta\Phi^\top \Phi + \alpha I) w - \beta t^\top \Phi w + \frac{\beta}{2}t^\top t. \end{aligned}$$

**Group terms in  $w$  and complete the square.** Write the quadratic form as

$$\frac{1}{2}w^\top A w - b^\top w + \text{const}, \quad \text{where } A = \beta\Phi^\top \Phi + \alpha I, \quad b = \beta\Phi^\top t.$$

Complete the square:

$$\frac{1}{2}w^\top A w - b^\top w = \frac{1}{2}(w - A^{-1}b)^\top A(w - A^{-1}b) - \frac{1}{2}b^\top A^{-1}b.$$

Thus the unnormalized posterior becomes

$$p(w | t) \propto \exp\left(-\frac{1}{2}(w - A^{-1}b)^\top A(w - A^{-1}b)\right) \cdot \exp\left(\frac{1}{2}b^\top A^{-1}b - \frac{\beta}{2}t^\top t\right).$$

The second exponential is independent of  $w$  and becomes part of the normalizing constant.

**Identify posterior covariance and mean.** Hence the posterior is Gaussian with precision  $A$  and covariance  $S_N = A^{-1}$ :

$$S_N = (\beta\Phi^\top \Phi + \alpha I)^{-1},$$

and posterior mean

$$m_N = A^{-1}b = (\beta\Phi^\top \Phi + \alpha I)^{-1}(\beta\Phi^\top t).$$

**Simplify using  $\lambda = \alpha/\beta$ .** Dividing numerator and denominator by  $\beta$  gives the more familiar form:

$$S_N = \beta^{-1}(\Phi^\top \Phi + \lambda I)^{-1}, \quad m_N = (\Phi^\top \Phi + \lambda I)^{-1}\Phi^\top t,$$

where  $\lambda = \alpha/\beta$ . Note that  $m_N$  equals the ridge/MAP estimator and  $S_N$  quantifies posterior uncertainty.